Optimisation proof FTLR Jmp/Jnz (#23)
* WIP factoring out proof FTLR jmp

* WIP factor out the part about IDC

* Remove useless arg in sub-buffer call_ie

* More general spec for jmp_to_unknown

* WIP factor out proof Jmp

* Slightly factor out proof FTLR Jmp and Jnz

* WIP

* WIP setup for close resource lemma FTLR Jmp

* Close invariants lemma for FTLR Jmp

* Setup for close resource lemma FTLR Jnz

* Close invariants lemma for FTLR Jnz

* Move lemmas where they belongs

* Tweak proof FTLR Jnz

* Factor out proof FTRL Jmp and Jnz: re-use setup from Jmp for Jnz

* Factor out proof WP rules Jmp and Jnz: re-use setup from jmp for jnz

theories/ftlr/Jmp.v
@@ -15,315 +15,337 @@ Section fundamental.
   Implicit Types w : (leibnizO Word).
   Implicit Types interp : (D).
 
+  (* The first part is common with Jnz. The argument =cond=
+     expresses the pure conditions specific to the kind of jump.
+   *)
 
   (* Mask after the jump, depending on the address of the pc and the address
    of a *)
-  Definition allow_jmp_mask (pc_a a : Addr) : coPset
+  Definition allow_jmp_mask (pc_a a a' : Addr) : coPset
     :=
     if decide (pc_a = a)
-    then (⊤ ∖ ↑logN.@pc_a ∖ ↑logN.@(a^+1)%a)
+    then (⊤ ∖ ↑logN.@pc_a ∖ ↑logN.@a')
     else
-      if decide (pc_a = (a^+1)%a)
+      if decide (pc_a = a')
       then (⊤ ∖ ↑logN.@pc_a ∖ ↑logN.@a)
-      else (⊤ ∖ ↑logN.@pc_a ∖ ↑logN.@a ∖ ↑logN.@(a^+1)%a).
+      else (⊤ ∖ ↑logN.@pc_a ∖ ↑logN.@a ∖ ↑logN.@a').
 
-  Definition allow_jmp_mask_reg (regs : Reg) (r : RegName) (pc_a : Addr) (p : Perm) (b e a : Addr)
+  Definition allow_jmp_mask_reg (cond : Prop) `{Decision cond} (regs : Reg) (r : RegName) (pc_a : Addr)
+    (p : Perm) (b e a : Addr)
     : coPset :=
-    if decide (reg_allows_IE_jmp regs r p b e a)
-    then allow_jmp_mask pc_a a
+    if decide (reg_allows_IE_jmp regs r p b e a /\ cond)
+    then allow_jmp_mask pc_a a (a ^+1)%a
     else (⊤ ∖ ↑logN.@pc_a).
 
   (* The necessary resources to close the region again,
      except for the points to predicate, which we will store separately *)
   Definition region_open_resources2
-    (pc_a : Addr) (a : Addr)
+    (pc_a : Addr) (a a' : Addr)
     (w1 : Word) (w2 : Word)
     (P1 P2 : D)
     : iProp Σ :=
     ▷ P1 w1 ∗ ▷ P2 w2
        ∗ persistent_cond P1 ∗ persistent_cond P2
-       ∗ ((▷ ∃ w1 w2, a ↦ₐ w1 ∗ P1 w1 ∗ (a^+1)%a ↦ₐ w2 ∗ P2 w2)
-          ={allow_jmp_mask pc_a a, ⊤ ∖ ↑logN.@pc_a}=∗ emp)%I.
+       ∗ ((▷ ∃ w1 w2, a ↦ₐ w1 ∗ P1 w1 ∗ a' ↦ₐ w2 ∗ P2 w2)
+          ={allow_jmp_mask pc_a a a', ⊤ ∖ ↑logN.@pc_a}=∗ emp)%I.
 
   Definition region_open_resources
-    (pc_a : Addr) (a : Addr) (w : Word)
+    (pc_a : Addr) (a a' : Addr) (w : Word)
     (P : D)
     : iProp Σ :=
     (▷ P w
        ∗ persistent_cond P
        ∗ ((▷ ∃ w, a ↦ₐ w ∗ P w)
-        ={allow_jmp_mask pc_a a, ⊤ ∖ ↑logN.@pc_a}=∗ emp))%I.
+        ={allow_jmp_mask pc_a a a', ⊤ ∖ ↑logN.@pc_a}=∗ emp))%I.
 
-  Definition region_open_resources'
-    (pc_a : Addr) (a : Addr) (w' : Word)
-    (P : D)
-    : iProp Σ :=
-    (▷ P w'
-       ∗ persistent_cond P
-       ∗ ((▷ ∃ w', (a^+1)%a ↦ₐ w' ∗ P w')
-        ={allow_jmp_mask pc_a a, ⊤ ∖ ↑logN.@pc_a}=∗ emp))%I.
+  Definition allow_jmp_res_mem
+    (pc_a : Addr) (a : Addr)
+    (P1 P2 : D): iProp Σ :=
+    (|={⊤ ∖ ↑logN.@pc_a, allow_jmp_mask pc_a a (a ^+1)%a}=>
+       (if decide (pc_a = a)
+        then ∃ w2, (a^+1)%a ↦ₐ w2 ∗ region_open_resources pc_a (a ^+1)%a a w2 P2
+        else
+          if decide (pc_a = (a^+1)%a)
+          then ∃ w1, a ↦ₐ w1 ∗ region_open_resources pc_a a (a ^+1)%a w1 P1
+          else ∃ w1 w2, a ↦ₐ w1 ∗ (a^+1)%a ↦ₐ w2 ∗ region_open_resources2 pc_a a (a ^+1)%a w1 w2 P1 P2)
+    )%I.
 
   (* Description of what the resources are supposed to look like after opening the
      region if we need to, but before closing the region up again*)
-  Definition allow_jmp_res (regs : Reg) (r : RegName)
+  Definition allow_jmp_res (cond : Prop) `{Decision cond} (regs : Reg) (r : RegName)
     (pc_a : Addr) (p : Perm) (b e a : Addr)
     (P1 P2 : D): iProp Σ :=
-    (⌜read_reg_inr regs r p b e a⌝ ∗
-
-       if decide (reg_allows_IE_jmp regs r p b e a)
+    (if decide (reg_allows_IE_jmp regs r p b e a /\ cond)
        then
-         (∀ w1 w2 regs', ▷ □ (P1 w1 ∗ (P2 w2 ∨ ⌜ is_int w2 ⌝)
-                              -∗ (interp_expr_gen interp regs' w1 w2)))
-           ∗
-           |={⊤ ∖ ↑logN.@pc_a, allow_jmp_mask pc_a a}=>
-           (if decide (pc_a = a)
-            then ∃ w2, (a^+1)%a ↦ₐ w2 ∗ region_open_resources' pc_a a w2 P2
-            else
-              if decide (pc_a = (a^+1)%a)
-              then ∃ w1, a ↦ₐ w1 ∗ region_open_resources pc_a a w1 P1
-              else ∃ w1 w2, a ↦ₐ w1 ∗ (a^+1)%a ↦ₐ w2 ∗ region_open_resources2 pc_a a w1 w2 P1 P2
-           )
+         (∀ w1 w2 regs', ▷ □ (P1 w1 ∗ (P2 w2 ∨ ⌜ is_int w2 ⌝) -∗ (interp_expr_gen interp regs' w1 w2)))
+           ∗ allow_jmp_res_mem pc_a a P1 P2
        else True)%I.
 
-  Lemma create_jmp_res:
+  Lemma create_jmp_res (cond : Prop) `{Decision cond}:
     ∀ (regs : leibnizO Reg) (r : RegName)
       (pc_p : Perm) (pc_b pc_e pc_a : Addr)
-      (widc : Word)
       (p : Perm) (b e a : Addr),
       pc_p <> IE ->
-      read_reg_inr (<[PC:=WCap pc_p pc_b pc_e pc_a]> (<[idc:= widc]> regs)) r p b e a
-      → (∀ (r' : RegName) (w : Word), ⌜r' ≠ PC⌝ → ⌜r' ≠ idc⌝ → ⌜regs !! r' = Some w⌝ → (fixpoint interp1) w)
-        -∗ interp widc
+      (∀ (r' : RegName) (w : Word), ⌜r' ≠ PC⌝ → ⌜regs !! r' = Some w⌝ → (fixpoint interp1) w)
         -∗ ∃ (P1 P2 : D),
-             allow_jmp_res (<[PC:=WCap pc_p pc_b pc_e pc_a]> (<[idc:=widc]> regs)) r pc_a p b e a P1 P2.
+             @allow_jmp_res cond _ (<[PC:=WCap pc_p pc_b pc_e pc_a]> regs) r pc_a p b e a P1 P2.
   Proof.
-    intros regs r pc_p pc_b pc_e pc_a widc p b e a Hpc_p HVr.
-    iIntros "#Hreg #Hwidc".
-    iFrame "%".
+    intros regs r pc_p pc_b pc_e pc_a p b e a Hpc_p.
+    iIntros "#Hreg".
+    rewrite /allow_jmp_res.
     case_decide as Hallows; cycle 1.
     - by iExists (λne _, True%I), (λne _, True%I).
     - rewrite /allow_jmp_mask.
-      destruct Hallows as (Hreg & -> & Hwb & Hwb').
+      destruct Hallows as [(Hreg & -> & Hwb & Hwb') Hcond].
       assert (a <> (a^+1)%a) by (apply Is_true_true_1, andb_prop in Hwb as [_ Hge]; solve_addr).
       assert ( withinBounds b e a /\ withinBounds b e (a^+1)%a) as Hwbs by auto.
 
       assert (r ≠ PC) as Hneq by (destruct (decide (r = PC)) ; simplify_map_eq; auto).
       rewrite lookup_insert_ne //= in Hreg.
 
-      (* TODO there are plenty of similar case, is there a way to factor out *)
+      iDestruct ("Hreg" $! r _ Hneq Hreg) as "Hvsrc".
+      rewrite fixpoint_interp1_eq /=.
+      iDestruct ("Hvsrc" $! Hwbs) as (P1 P2) "(Hpers_P1 & Hpers_P2 & Hinv_a & Hinv_a' & Hexec)".
+      iExists P1, P2.
+      iFrame "#".
+      iClear "Hexec".
+      rewrite /allow_jmp_res_mem.
+
       case_decide as Ha; simplify_eq.
-      {
-        destruct (decide (r = idc)) as [|Hneq']; simplify_map_eq.
-        + rewrite fixpoint_interp1_eq /=.
-          iDestruct ("Hwidc" $! Hwbs) as (P1 P2) "(Hpers_P1 & Hpers_P2 & Hinv_a & Hinv_a' & Hexec)".
-          iExists P1, P2.
-          iFrame "#".
-          iMod (inv_acc (⊤ ∖ ↑logN.@a) with "Hinv_a'") as "[Hrefinv_a' Hcls_a']";[solve_ndisj|].
-          iDestruct "Hrefinv_a'" as (w2) "[>Ha' HPa']".
-          iExists w2.
-          iFrame "∗ #".
-          rewrite /allow_jmp_mask. do 2 (case_decide ; solve_addr).
-        + iDestruct ("Hreg" $! r _ Hneq Hneq' Hreg) as "Hvsrc".
-          rewrite (fixpoint_interp1_eq (WCap _ _ _ _)) /=.
-          iDestruct ("Hvsrc" $! Hwbs) as (P1 P2) "(Hpers_P1 & Hpers_P2 & Hinv_a & Hinv_a' & Hexec)".
-          iExists P1, P2.
-          iFrame "#".
-          iMod (inv_acc (⊤ ∖ ↑logN.@a) with "Hinv_a'") as "[Hrefinv_a' Hcls_a']";[solve_ndisj|].
-          iDestruct "Hrefinv_a'" as (w2) "[>Ha' HPa']".
-          iExists w2.
-          iFrame "∗ #".
-          rewrite /allow_jmp_mask. do 2 (case_decide ; solve_addr).
+      { (* pc_a = a *)
+        iMod (inv_acc (⊤ ∖ ↑logN.@a) with "Hinv_a'") as "[Hrefinv_a' Hcls_a']";[solve_ndisj|].
+        iDestruct "Hrefinv_a'" as (w2) "[>Ha' HPa']".
+        iExists w2.
+        iFrame "∗ #".
+        rewrite /allow_jmp_mask decide_True //= decide_False //= decide_True //=.
       }
 
       case_decide as Ha'; simplify_eq.
-      {
-        destruct (decide (r = idc)) as [|Hneq']; simplify_map_eq.
-        + rewrite fixpoint_interp1_eq /=.
-          iDestruct ("Hwidc" $! Hwbs) as (P1 P2) "(Hpers_P1 & Hpers_P2 & Hinv_a & Hinv_a' & Hexec)".
-          iExists P1, P2.
-          iFrame "#".
-          iMod (inv_acc (⊤ ∖ ↑logN.@(a ^+ 1)%a) with "Hinv_a") as "[Hrefinv_a Hcls_a]";[solve_ndisj|].
-          iDestruct "Hrefinv_a" as (w1) "[>Ha HPa]".
-          iExists w1.
-          iFrame "∗ #".
-          rewrite /allow_jmp_mask. do 2 (case_decide ; try solve_addr).
-        + iDestruct ("Hreg" $! r _ Hneq Hneq' Hreg) as "Hvsrc".
-          rewrite (fixpoint_interp1_eq (WCap _ _ _ _)) /=.
-          iDestruct ("Hvsrc" $! Hwbs) as (P1 P2) "(Hpers_P1 & Hpers_P2 & Hinv_a & Hinv_a' & Hexec)".
-          iExists P1, P2.
-          iFrame "#".
-          iMod (inv_acc (⊤ ∖ ↑logN.@(a ^+ 1)%a) with "Hinv_a") as "[Hrefinv_a Hcls_a]";[solve_ndisj|].
-          iDestruct "Hrefinv_a" as (w1) "[>Ha HPa]".
-          iExists w1.
-          iFrame "∗ #".
-          rewrite /allow_jmp_mask. do 2 (case_decide ; try solve_addr).
+      { (* pc_a = a+1 *)
+        iMod (inv_acc (⊤ ∖ ↑logN.@(a ^+ 1)%a) with "Hinv_a") as "[Hrefinv_a Hcls_a]";[solve_ndisj|].
+        iDestruct "Hrefinv_a" as (w2) "[>Ha HPa]".
+        iExists w2.
+        iFrame "∗ #".
+        rewrite /allow_jmp_mask decide_False //= decide_True //=.
       }
 
-      destruct (decide (r = idc)) as [|Hneq']; simplify_map_eq.
-      + rewrite fixpoint_interp1_eq /=.
-        iDestruct ("Hwidc" $! Hwbs) as (P1 P2) "(Hpers_P1 & Hpers_P2 & Hinv_a & Hinv_a' & Hexec)".
-        iExists P1, P2.
+      (* pc_a ≠ a ∧ pc_a ≠ a+1 *)
+      iMod (inv_acc (⊤ ∖ ↑logN.@pc_a) with "Hinv_a") as "[Hrefinv_a Hcls_a]";[solve_ndisj|].
+      iMod (inv_acc (⊤ ∖ ↑logN.@pc_a ∖ ↑logN.@a) with "Hinv_a'") as "[Hrefinv_a' Hcls_a']";[solve_ndisj|].
+      iDestruct "Hrefinv_a" as (w1) "[>Ha HPa]".
+      iDestruct "Hrefinv_a'" as (w2) "[>Ha' HPa']".
+      iExists w1, w2.
 
-        iFrame "#".
-        iMod (inv_acc (⊤ ∖ ↑logN.@pc_a) with "Hinv_a") as "[Hrefinv_a Hcls_a]";[solve_ndisj|].
-        iMod (inv_acc (⊤ ∖ ↑logN.@pc_a ∖ ↑logN.@a) with "Hinv_a'") as "[Hrefinv_a' Hcls_a']";[solve_ndisj|].
-        iDestruct "Hrefinv_a" as (w1) "[>Ha HPa]".
-        iDestruct "Hrefinv_a'" as (w2) "[>Ha' HPa']".
-        iExists w1, w2.
-
-        iFrame "∗ #".
-        rewrite /region_open_resources2.
-        iModIntro.
-        iIntros "Ha".
-        iDestruct "Ha" as (w1' w2') "(Hw1' & HP1' & Hw2' & HP2')".
-        rewrite /allow_jmp_mask.
-        case_decide; simplify_eq.
-        case_decide; simplify_eq.
-        iMod ("Hcls_a'" with "[Hw2' HP2']") as "_"; first (iExists _ ; iFrame).
-        iMod ("Hcls_a" with "[Hw1' HP1']") as "_"; first (iExists _ ; iFrame).
-        done.
-      + iDestruct ("Hreg" $! r _ Hneq Hneq' Hreg) as "Hvsrc".
-        rewrite (fixpoint_interp1_eq (WCap _ _ _ _)) /=.
-        iDestruct ("Hvsrc" $! Hwbs) as (P1 P2) "(Hpers_P1 & Hpers_P2 & Hinv_a & Hinv_a' & Hexec)".
-        iExists P1, P2.
-
-        iFrame "#".
-        iMod (inv_acc (⊤ ∖ ↑logN.@pc_a) with "Hinv_a") as "[Hrefinv_a Hcls_a]";[solve_ndisj|].
-        iMod (inv_acc (⊤ ∖ ↑logN.@pc_a ∖ ↑logN.@a) with "Hinv_a'") as "[Hrefinv_a' Hcls_a']";[solve_ndisj|].
-        iDestruct "Hrefinv_a" as (w1) "[>Ha HPa]".
-        iDestruct "Hrefinv_a'" as (w2) "[>Ha' HPa']".
-        iExists w1, w2.
-
-        iFrame "∗ #".
-        rewrite /region_open_resources2.
-        iModIntro.
-        iIntros "Ha".
-        iDestruct "Ha" as (w1' w2') "(Hw1' & HP1' & Hw2' & HP2')".
-        rewrite /allow_jmp_mask.
-        case_decide; simplify_eq.
-        case_decide; simplify_eq.
-        iMod ("Hcls_a'" with "[Hw2' HP2']") as "_"; first (iExists _ ; iFrame).
-        iMod ("Hcls_a" with "[Hw1' HP1']") as "_"; first (iExists _ ; iFrame).
-        done.
+      rewrite /region_open_resources2 /allow_jmp_mask decide_False //= decide_False //=.
+      iFrame "∗ #".
+      iModIntro.
+      iIntros "Ha".
+      iDestruct "Ha" as (w1' w2') "(Hw1' & HP1' & Hw2' & HP2')".
+      iMod ("Hcls_a'" with "[Hw2' HP2']") as "_"; first (iExists _ ; iFrame).
+      iMod ("Hcls_a" with "[Hw1' HP1']") as "_"; first (iExists _ ; iFrame).
+      done.
   Qed.
 
-  Definition allow_jmp_mem
+  Definition allow_jmp_mem_res
+    (mem : Mem) (pc_a : Addr) (pc_w : Word) (a : Addr) (P1 P2 : D) :=
+    (if decide (pc_a = a)
+    then ∃ w2, ⌜mem = <[(a^+1)%a:=w2]> (<[pc_a:=pc_w]> ∅)⌝ ∗ region_open_resources pc_a (a^+1)%a a w2 P2
+    else
+      if decide (pc_a = (a^+1)%a)
+      then ∃ w1, ⌜mem = <[a:=w1]> (<[pc_a:=pc_w]> ∅)⌝ ∗ region_open_resources pc_a a (a^+1)%a w1 P1
+      else ∃ w1 w2,
+          ⌜mem = <[(a^+1)%a:=w2]> (<[a:=w1]> (<[pc_a:=pc_w]> ∅))⌝ ∗ region_open_resources2 pc_a a (a^+1)%a w1 w2 P1 P2)%I.
+
+  Definition allow_jmp_mem (cond : Prop) `{Decision cond}
     (regs : Reg) (mem : Mem) (r : RegName)
     (pc_a : Addr) (pc_w : Word) (p : Perm) (b e a : Addr) (P1 P2 : D) :=
-    (⌜read_reg_inr regs r p b e a⌝ ∗
-       if decide (reg_allows_IE_jmp regs r p b e a)
-       then (if decide (pc_a = a)
-             then ∃ w2, ⌜mem = <[(a^+1)%a:=w2]> (<[pc_a:=pc_w]> ∅)⌝ ∗ region_open_resources' pc_a a w2 P2
-             else
-               if decide (pc_a = (a^+1)%a)
-               then ∃ w1, ⌜mem = <[a:=w1]> (<[pc_a:=pc_w]> ∅)⌝ ∗ region_open_resources pc_a a w1 P1
-               else ∃ w1 w2,
-                   ⌜mem = <[(a^+1)%a:=w2]> (<[a:=w1]> (<[pc_a:=pc_w]> ∅))⌝
-                                             ∗ region_open_resources2 pc_a a w1 w2 P1 P2)
+    (if decide (reg_allows_IE_jmp regs r p b e a /\ cond)
+       then allow_jmp_mem_res mem pc_a pc_w a P1 P2
        else ⌜mem = <[pc_a:=pc_w]> ∅⌝)%I.
 
-  Lemma jmp_res_implies_mem_map:
+  Lemma jmp_res_implies_mem_map (cond : Prop) `{Decision cond}:
     ∀ (regs : leibnizO Reg) (r : RegName)
       (pc_a : Addr) (pc_w : Word)
       (p : Perm) (b e a: Addr)
       (P1 P2:D),
-      allow_jmp_res regs r pc_a p b e a P1 P2
+      read_reg_inr regs r p b e a
+      -> @allow_jmp_res cond _ regs r pc_a p b e a P1 P2
       -∗ pc_a ↦ₐ pc_w
-      ={⊤ ∖ ↑logN.@pc_a, allow_jmp_mask_reg regs r pc_a p b e a}=∗
+      ={⊤ ∖ ↑logN.@pc_a, @allow_jmp_mask_reg cond _ regs r pc_a p b e a }=∗
       ∃ mem : Mem,
-          allow_jmp_mem regs mem r pc_a pc_w p b e a P1 P2
+          @allow_jmp_mem cond _ regs mem r pc_a pc_w p b e a P1 P2
             ∗ ▷ ([∗ map] a0↦w ∈ mem, a0 ↦ₐ w).
   Proof.
-    intros regs r pc_a pc_w p b e a P1 P2.
+    intros regs r pc_a pc_w p b e a P1 P2 Hrinr.
     iIntros "HJmpRes Hpc_a".
-    iDestruct "HJmpRes" as "[%Hrinr HJmpRes]".
-    rewrite /allow_jmp_mask /allow_jmp_mask_reg.
+    rewrite /allow_jmp_res /allow_jmp_mask /allow_jmp_mask_reg.
 
     case_decide as Hdec ; cycle 1.
     { rewrite /read_reg_inr in Hrinr.
       iExists _.
       iSplitL "HJmpRes".
-      + iModIntro. rewrite /allow_jmp_mem. iSplitR; auto.
-        case_decide; first by exfalso. auto.
+      + rewrite /allow_jmp_mem decide_False //=.
       + iModIntro. iNext. by iApply memMap_resource_1.
     }
-    destruct Hdec as (Hreg & -> & Hwb & Hwb').
+    destruct Hdec as [(Hreg & -> & Hwb & Hwb') Hcond].
     assert (a <> (a^+1)%a) as Haeq by (apply Is_true_true_1, andb_prop in Hwb as [_ Hge]; solve_addr).
-    rewrite /allow_jmp_mask.
     iDestruct "HJmpRes" as "[Hexec HJmpRes]".
     iMod "HJmpRes" as "HJmpRes".
+    rewrite /allow_jmp_mask /allow_jmp_mem /allow_jmp_mem_res.
 
     case_decide as Ha ; simplify_eq.
     { (* pc_a = a *)
       iDestruct "HJmpRes" as (w2) "[Ha' HJmpRest]".
       iExists _.
-      iSplitL "HJmpRest".
-      + iSplitR; first auto.
-
-        case_decide as Hdec1.
-        2: {
-          apply not_and_r in Hdec1 as [Hcontra|Hcontra]; simplify_eq.
-          exfalso; apply Hcontra ; repeat (split ; auto).
-        }
-        case_decide; simplify_eq; auto.
-      + iModIntro. iNext.
-        rewrite memMap_resource_2ne; auto; iFrame.
+      iModIntro.
+      rewrite decide_True; [|by rewrite /reg_allows_IE_jmp].
+      iSplitL "HJmpRest"; eauto.
+      iNext ; rewrite memMap_resource_2ne; auto; iFrame.
     }
-    (* pc_a ≠ a *)
+
     case_decide as Ha' ; simplify_eq.
     { (* pc_a = a+1 *)
       iDestruct "HJmpRes" as (w1) "[Ha HJmpRest]".
       iExists _.
-      iSplitL "HJmpRest".
-      + iSplitR; first auto.
-        case_decide as Hdec1.
-        2: {
-          apply not_and_r in Hdec1 as [Hcontra|Hcontra]; simplify_eq.
-          exfalso; apply Hcontra ; repeat (split ; auto).
-        }
-        case_decide; simplify_eq; auto.
-        case_decide; simplify_eq; auto.
-      + iModIntro. iNext.
-        rewrite memMap_resource_2ne; auto; iFrame.
+      iModIntro.
+      rewrite decide_True; [|by rewrite /reg_allows_IE_jmp].
+      iSplitL "HJmpRest"; eauto.
+      iNext ; rewrite memMap_resource_2ne; auto; iFrame.
     }
-    (* pc_a ≠ a+1 *)
 
+    (* pc_a ≠ a ∧ pc_a ≠ a+1 *)
     iDestruct "HJmpRes" as (w1 w2) "(Ha & Ha' & HJmpRest)".
     iExists _.
-    iSplitL "HJmpRest".
-    + iSplitR; first auto.
-      case_decide as Hdec1.
-      2: {
-        apply not_and_r in Hdec1 as [Hcontra|Hcontra]; simplify_eq.
-        exfalso; apply Hcontra ; repeat (split ; auto).
-      }
-      case_decide; simplify_eq; auto.
-      case_decide; simplify_eq; auto.
-    + iModIntro. iNext.
-      rewrite memMap_resource_3ne; auto; iFrame.
+    iModIntro.
+    rewrite decide_True; [|by rewrite /reg_allows_IE_jmp].
+    iSplitL "HJmpRest"; eauto.
+    iNext ; rewrite memMap_resource_3ne; auto; iFrame.
   Qed.
 
+  (* Close the invariants, in case of fail*)
+  Lemma mem_map_recover_res
+    (mem : Mem) (pc_a a : Addr) (pc_w : Word) (P1 P2 : D):
+    (a ^+ 1)%a ≠ a ->
+    allow_jmp_mem_res mem pc_a pc_w a P1 P2
+    -∗ ([∗ map] a'↦w' ∈ mem, a' ↦ₐ w')
+    ={allow_jmp_mask pc_a a (a ^+1)%a, ⊤ ∖ ↑logN.@pc_a}=∗ pc_a ↦ₐ pc_w.
+  Proof.
+    iIntros (Hneq) "HJmpMem Hmem".
+
+    rewrite /allow_jmp_mem_res /allow_jmp_mask.
+    case_decide as Ha; simplify_eq.
+    { (* pc_a = a *)
+      iDestruct "HJmpMem" as (w2) "(->&Hres)". rewrite /region_open_resources.
+      rewrite memMap_resource_2ne; auto.
+      iDestruct "Hmem" as "(Ha0' & Ha0)".
+      iDestruct "Hres" as "(HP2 & _ & Hcls')".
+      rewrite /allow_jmp_mask.
+      rewrite decide_False //= decide_True //=.
+      iMod ("Hcls'" with "[HP2 Ha0']") as "_" ; [iNext ; iExists w2; iFrame|auto].
+    }
+
+    case_decide as Ha'; simplify_eq.
+    { (* pc_a = a+1 *)
+      iDestruct "HJmpMem" as (w1) "(->&Hres)". rewrite /region_open_resources.
+      rewrite memMap_resource_2ne; auto.
+      iDestruct "Hmem" as "(Ha0 & Ha0')".
+      iDestruct "Hres" as "(HP1 & _ & Hcls')".
+      rewrite /allow_jmp_mask.
+      rewrite decide_False //= decide_True //=.
+      iMod ("Hcls'" with "[HP1 Ha0]") as "_" ; [iNext ; iExists w1; iFrame|auto].
+    }
+
+    (* a ≠ a0 ∧ a ≠ a0+1 *)
+    iDestruct "HJmpMem" as (w1 w2) "(->&Hres)". rewrite /region_open_resources2.
+    rewrite memMap_resource_3ne; auto.
+    iDestruct "Hmem" as "(Ha0' & Ha0 & Ha)".
+    iDestruct "Hres" as "(HP1 & HP2 & _& _ & Hcls')".
+    rewrite /allow_jmp_mask.
+    rewrite decide_False //= decide_False //=.
+    iMod ("Hcls'" with "[HP1 HP2 Ha0 Ha0']") as "_"; [iNext ; iExists w1,w2; iFrame|auto].
+  Qed.
+
+  (* Close the invariants, in case of jump to IE *)
+  Lemma mem_map_recover_res_ie
+    (mem : Mem) (pc_a a : Addr) (pc_w wpc widc : Word) (P P1 P2 : D):
+    (a ^+ 1)%a ≠ a ->
+    mem !! a = Some wpc ->
+    mem !! (a ^+ 1)%a = Some widc ->
+
+    allow_jmp_mem_res mem pc_a pc_w a P1 P2
+    -∗ ([∗ map] a'↦w' ∈ mem, a' ↦ₐ w')
+    ={allow_jmp_mask pc_a a (a ^+1)%a, ⊤ ∖ ↑logN.@pc_a}=∗
+      if (decide (pc_a = a))
+      then pc_a ↦ₐ pc_w ∗ ⌜pc_w = wpc ⌝
+      else
+        if (decide (pc_a = (a^+1)%a))
+        then pc_a ↦ₐ widc ∗ ⌜pc_w = widc⌝ ∗ ▷ P1 wpc ∗ persistent_cond P1
+        else pc_a ↦ₐ pc_w ∗ ▷ P1 wpc ∗ ▷ P2 widc ∗ persistent_cond P1 ∗ persistent_cond P2.
+  Proof.
+    iIntros (Hneq Hmem_a Hmem_a') "HJmpMem Hmem".
+    rewrite /allow_jmp_mem_res /allow_jmp_mask.
+
+    case_decide as Ha; simplify_eq.
+    { (* a = a0 *)
+      iDestruct "HJmpMem" as (w2) "(->& HP2& %Hpers2& Hcls')".
+      rewrite /allow_jmp_mask.
+      rewrite decide_False //= decide_True //=.
+      rewrite memMap_resource_2ne; auto.
+      simplify_map_eq.
+      iDestruct "Hmem" as  "[Ha0' Ha0]".
+      iMod ("Hcls'" with "[HP2 Ha0']") as "_" ; [iNext;iExists widc;iFrame "∗ #"|auto].
+    }
+
+    case_decide as Ha'; simplify_eq.
+    { (* a = a0+1 *)
+      iDestruct "HJmpMem" as (w1) "(->& HP1& %Hpers1& Hcls')".
+      iDestruct "HP1" as "#HP1".
+      rewrite /allow_jmp_mask.
+      rewrite decide_False //= decide_True //=.
+      rewrite memMap_resource_2ne; auto.
+      simplify_map_eq.
+      iDestruct "Hmem" as "[Ha0' Ha0]".
+      iMod ("Hcls'" with "[HP1 Ha0']") as "_" ; [iNext;iExists wpc;iFrame "∗ #"|auto].
+    }
+
+    (* a ≠ a0 ∧ a ≠ a0+1 *)
+    iDestruct "HJmpMem" as (w1 w2) "(->& HP1& HP2& %Hpers1& %Hpers2& Hcls')".
+    rewrite /region_open_resources2.
+    iDestruct "HP1" as "#HP1"; iDestruct "HP2" as "#HP2".
+    rewrite /allow_jmp_mask; case_decide ; simplify_eq; case_decide ; simplify_eq.
+    rewrite memMap_resource_3ne; auto.
+    simplify_map_eq.
+    iDestruct "Hmem" as  "(Ha0' & Ha0 & Ha)".
+    iMod ("Hcls'" with "[HP1 HP2 Ha0' Ha0]") as "_"; [iNext;iExists wpc,widc;iFrame "∗ #"|auto].
+  Qed.
+
+  (* Derice pure conds =allow_jmp_mmap_or_true= from =cond_jmp= *)
   Lemma mem_map_implies_pure_conds:
     ∀ (regs : leibnizO Reg) (mem : Mem) (r : RegName)
       (pc_a : Addr) (pc_w : Word)
       (p : Perm) (b e a : Addr) (P1 P2 : D),
-      allow_jmp_mem regs mem r pc_a pc_w p b e a P1 P2
-        -∗ ⌜mem !! pc_a = Some pc_w⌝
-          ∗ ⌜allow_jmp_mmap_or_true r regs mem⌝.
+      read_reg_inr regs r p b e a
+      -> allow_jmp_mem cond_jmp regs mem r pc_a pc_w p b e a P1 P2
+      -∗ ⌜mem !! pc_a = Some pc_w⌝ ∗ ⌜allow_jmp_mmap_or_true cond_jmp r regs mem⌝.
   Proof.
-    iIntros (regs mem r pc_a pc_w p b e a P1 P2) "HJmpMem".
-    iDestruct "HJmpMem" as "[%Hrinr HJmpRes]".
+    iIntros (regs mem r pc_a pc_w p b e a P1 P2 Hrinr) "HJmpMem".
+    rewrite /allow_jmp_mem.
     case_decide as Hdec ; cycle 1.
-    { iDestruct "HJmpRes" as "->".
+    { iDestruct "HJmpMem" as "->".
       iSplitR. by rewrite lookup_insert.
       iExists p,b,e,a.
       iSplitR; auto.
-      case_decide as Hdec1; auto.
+      rewrite decide_False //=.
     }
+    destruct Hdec as [Hdec _].
+
+    rewrite /allow_jmp_mem_res.
     assert (a <> (a^+1)%a)
     by (inversion Hdec as (_ & _ & Hwb%Is_true_true_1%withinBounds_true_iff & _); solve_addr).
+
     case_decide as Ha; simplify_eq.
-    { iDestruct "HJmpRes" as (w2) "[%Hmem _]" ; subst.
+    { (* pc_a = a *)
+      iDestruct "HJmpMem" as (w2) "[%Hmem _]" ; subst.
       iSplitL.
       by iPureIntro; simplify_map_eq.
       iExists p,b,e,a.
@@ -333,8 +355,10 @@ Section fundamental.
       iExists pc_w, w2.
       by iPureIntro ; split ; simplify_map_eq.
     }
+
     case_decide as Ha'; simplify_eq.
-    { iDestruct "HJmpRes" as (w1) "[%Hmem _]" ; subst.
+    { (* pc_a = a+1 *)
+      iDestruct "HJmpMem" as (w1) "[%Hmem _]" ; subst.
       iSplitL.
       by iPureIntro; simplify_map_eq.
       iExists p,b,e,a.
@@ -345,7 +369,8 @@ Section fundamental.
       by iPureIntro ; split ; simplify_map_eq.
     }
 
-    iDestruct "HJmpRes" as (w1 w2) "[%Hmem _]" ; subst.
+    (* pc_a ≠ a ∧ pc_a ≠ a+1 *)
+    iDestruct "HJmpMem" as (w1 w2) "[%Hmem _]" ; subst.
     iSplitL.
     by iPureIntro; simplify_map_eq.
     iExists p,b,e,a.
@@ -354,18 +379,6 @@ Section fundamental.
     inversion Hdec.
     iExists w1, w2.
     by iPureIntro ; split ; simplify_map_eq.
-  Qed.
-
-  Lemma reg_allows_IE_jmp_same
-    (regs : Reg) (r : RegName)
-    (p p' : Perm) (b b' e e' a a' : Addr):
-    reg_allows_IE_jmp regs r p b e a ->
-    regs !! r = Some (WCap p' b' e' a') ->
-    (p = p' /\ b = b' /\ e = e' /\ a = a').
-  Proof.
-    intros HallowJmp Hregs.
-    destruct HallowJmp as (Hregs'&->&_).
-    by rewrite Hregs' in Hregs; simplify_eq.
   Qed.
 
   Lemma jmp_case (regs : leibnizO Reg) (p : Perm)
@@ -399,27 +412,35 @@ Section fundamental.
       by repeat eexists.
     }
 
+    iAssert (∀ (r' : RegName) (w : Word),
+                ⌜r' ≠ PC⌝ → ⌜<[idc:=widc]> regs  !! r' = Some w⌝ → fixpoint interp1 w)%I
+      as "Hreg'".
+    { iIntros.
+      destruct (decide (r' = idc)); simplify_map_eq; auto.
+      iApply "Hreg";eauto.
+    }
+
     (* Step 1: open the region, if necessary, and store all the resources
        obtained from the region in allow_IE_res *)
-    iDestruct (create_jmp_res with "Hreg Hinv_idc") as (P1 P2) "HJmpRes"; eauto.
-    { destruct Hp ; destruct p ; auto. }
+    iDestruct ((create_jmp_res cond_jmp _ _ p)  with "Hreg'") as (P1 P2) "HJmpRes"; eauto.
+    { destruct Hp ; destruct p ; eauto. }
 
     (* Step2: derive the concrete map of memory we need, and any spatial
        predicates holding over it *)
-    iMod (jmp_res_implies_mem_map with "HJmpRes Ha") as (mem) "[HJmpMem HJmpRest]".
+    iMod ((jmp_res_implies_mem_map cond_jmp) with "HJmpRes Ha") as (mem) "[HJmpMem HJmpRest]"; first eauto.
 
     (* Step 3:  derive the non-spatial conditions over the memory map*)
     iDestruct (mem_map_implies_pure_conds with "HJmpMem") as
       %(HReadPC & HAJmpMem); auto.
 
     (* Step 3.5:  derive the non-spatial conditions over the registers *)
-    iAssert (⌜allow_jmp_rmap_or_true src
-               (<[PC:=WCap p b e a]> (<[idc:=widc]> regs))⌝)%I as "%HAJmpReg".
+    assert (allow_jmp_rmap_or_true cond_jmp src
+               (<[PC:=WCap p b e a]> (<[idc:=widc]> regs))) as HAJmpReg.
     { rewrite /allow_jmp_rmap_or_true.
-      iExists p0, b0, e0, a0.
-      iSplit; auto.
+      exists p0, b0, e0, a0.
+      split; auto.
       case_decide as Heq; auto.
-      by iExists widc; simplify_map_eq.
+      by exists widc; simplify_map_eq.
     }
 
     iApply (wp_jmp with "[Hmap HJmpRest]");eauto.
@@ -427,114 +448,90 @@ Section fundamental.
     { rewrite /subseteq /map_subseteq /set_subseteq_instance. intros rr _.
       apply elem_of_dom. repeat (rewrite lookup_insert_is_Some'; right); eauto. }
     { iSplitR "Hmap"; auto. }
+
     iNext. iIntros (regs' retv). iDestruct 1 as (HSpec) "[Hmem Hmap]".
     (* Infer that if P holds at w, then w must be valid (read condition) *)
     iDestruct ("Hread" with "HP") as "#Hw".
-    rewrite /allow_jmp_res /allow_jmp_mem /allow_jmp_mask_reg /allow_jmp_mask.
 
     destruct HSpec as [* Hregs Hwb Hwb' Ha Ha' HincrPC | * Hregs HnIE HincrPC | Hfail].
-    - (* succes jmp IE *)
+    - (* success jmp IE *)
       rewrite insert_insert insert_commute //= insert_insert in HincrPC; subst regs'.
-      destruct (decide (reg_allows_IE_jmp
-                          (<[PC:=WCap p b e a]> (<[idc:=widc]> regs))
-                          src p0 b0 e0 a0)) as [HallowJmp|HallowJmp].
-      2: { (* contradiction *)
-        rewrite /reg_allows_IE_jmp in HallowJmp.
-        rewrite /read_reg_inr in HVsrc.
-        rewrite Hregs in HVsrc; simplify_eq.
-        repeat (apply not_and_r in HallowJmp as [HallowJmp|HallowJmp] ; simplify_eq)
-        ;congruence.
-      }
-      assert (PC <> src) as Hsrc
-          by (destruct (decide (PC = src)); auto; simplify_map_eq; by destruct Hp).
-      assert (p0 = IE /\ b0 = b1 /\ e0 = e1 /\ a0 = a1) as (-> & -> & -> & ->)
-          by (by eapply reg_allows_IE_jmp_same)
-      ; simplify_map_eq.
-      assert ((a1 ^+ 1)%a ≠ a1) as Haeq by (apply Is_true_true_1, withinBounds_true_iff in Hwb ; solve_addr).
-      assert (withinBounds b1 e1 a1 ∧ withinBounds b1 e1 (a1 ^+ 1)%a) as Hbounds by auto.
 
-      iDestruct "HJmpMem" as "(_&HJmpMem)".
-      iDestruct "HJmpRes" as "(_&Hexec&HJmpRes)".
+      assert (p0 = IE /\ b0 = b1 /\ e0 = e1 /\ a0 = a1) as (-> & <- & <- & <-)
+          by (by rewrite /read_reg_inr in HVsrc; rewrite Hregs in HVsrc; simplify_eq).
+      assert ((a0 ^+ 1)%a ≠ a0) as Haeq by (apply Is_true_true_1, withinBounds_true_iff in Hwb ; solve_addr).
+      assert (withinBounds b0 e0 a0 ∧ withinBounds b0 e0 (a0 ^+ 1)%a) as Hbounds by auto.
+      assert (PC <> src) as Hsrc
+          by (destruct (decide (PC = src)); auto; simplify_map_eq; by
+                destruct Hp).
+      assert (reg_allows_IE_jmp
+                (<[PC:=WCap p b e a]> (<[idc:=widc]> regs))
+                src IE b0 e0 a0) as HallowJmp
+          by (by rewrite /reg_allows_IE_jmp; auto).
+
+      rewrite /allow_jmp_res /allow_jmp_mask_reg.
+      rewrite !decide_True //=.
+      iDestruct "HJmpRes" as "(Hexec&HJmpRes)".
+      rewrite /allow_jmp_mem.
+      rewrite !decide_True //=.
+
+      (* Step 4: return all the resources we had *)
+      iMod ((mem_map_recover_res_ie _ _ _ w wpc widc0 P P1 P2) with "HJmpMem Hmem") as "Ha"
+      ; auto; iModIntro.
+
       case_decide as Ha0; simplify_eq.
       { (* a = a0 *)
 
-        iDestruct "HJmpMem" as (w2) "(->& HP2& %Hpers2& Hcls')".
-        iDestruct "HP2" as "#HP2".
-        rewrite /allow_jmp_mask.
-        case_decide ; simplify_eq.
-        rewrite memMap_resource_2ne; auto.
-        simplify_map_eq.
+        iDestruct "Ha" as "[Ha0 ->]".
 
-        iDestruct "Hmem" as  "[Ha0' Ha0]".
-        iMod ("Hcls'" with "[HP2 Ha0']") as "_"; [iNext;iExists widc0;iFrame "∗ #"|iModIntro].
         iMod ("Hcls" with "[HP Ha0]") as "_"; [iNext;iExists wpc;iFrame|iModIntro].
-        iClear "HJmpRes".
         iApply wp_pure_step_later; auto.
         iNext ; iIntros "_".
         destruct wpc; cbn in Hi; try done.
         iExtract "Hmap" PC as "HPC".
         iApply interp_expr_invalid_pc; try iFrame ; eauto.
-        intro Hcontra; inversion Hcontra.
+        intro Hcontra; inversion Hcontra ; simplify_eq.
         iPureIntro; apply regmap_full_dom in Hsome; rewrite -Hsome; set_solver.
       }
 
-      (* a ≠ a0 *)
       case_decide as Ha0'; simplify_eq.
       { (* a = a0+1 *)
 
-        iDestruct "HJmpMem" as (w1) "(->& HP1& %Hpers1& Hcls')".
+        iDestruct "Ha" as "(Ha0 & -> & HP1 & %Hpers1)".
         iDestruct "HP1" as "#HP1".
-        rewrite /allow_jmp_mask.
-        case_decide ; simplify_eq.
-        case_decide ; simplify_eq.
-        rewrite memMap_resource_2ne; auto.
-        simplify_map_eq.
 
-        iDestruct "Hmem" as  "[Ha0' Ha0]".
-        iMod ("Hcls'" with "[HP1 Ha0']") as "_"; [iNext;iExists wpc;iFrame "∗ #"|iModIntro].
         iMod ("Hcls" with "[HP Ha0]") as "_"; [iNext;iExists widc0;iFrame|iModIntro].
-        iClear "HJmpRes".
         iApply wp_pure_step_later; auto.
         iNext ; iIntros "_".
-
         iApply ("Hexec" $! _ widc0) ; iFrame "∗ #".
         iRight; destruct widc0; cbn in Hi; try done.
-
         rewrite insert_commute //=.
         repeat (iSplit ; try done).
       }
 
-      (* a ≠ a0+1 *)
-      iDestruct "HJmpMem" as (w1 w2) "(->& HP1& HP2& %Hpers1& %Hpers2& Hcls')".
-      rewrite /region_open_resources2.
+      (* a ≠ a0 ∧ a ≠ a0+1 *)
+      iDestruct "Ha" as "(Ha & HP1 & HP2 & %Hpers1 & %Hpers2)".
       iDestruct "HP1" as "#HP1"; iDestruct "HP2" as "#HP2".
-      rewrite /allow_jmp_mask; case_decide ; simplify_eq; case_decide ; simplify_eq.
-      rewrite memMap_resource_3ne; auto.
-      simplify_map_eq.
-
-      iDestruct "Hmem" as  "(Ha0' & Ha0 & Ha)".
-      iMod ("Hcls'" with "[HP1 HP2 Ha0' Ha0]") as "_"; [iNext;iExists wpc,widc0;iFrame "∗ #"|iModIntro].
       iMod ("Hcls" with "[HP Ha]") as "_"; [iNext;iExists w;iFrame|iModIntro].
-      iClear "HJmpRes".
       iApply wp_pure_step_later; auto.
       iNext; iIntros "_".
-
       iApply "Hexec" ; iFrame "∗ #".
       rewrite insert_commute //=.
       repeat (iSplit ; try done).
 
     - (* success jmp not IE *)
       rewrite insert_insert in HincrPC; subst regs'.
-      destruct (decide (reg_allows_IE_jmp
+      rewrite /allow_jmp_mask_reg /allow_jmp_mem /allow_jmp_res.
+      destruct (decide ((reg_allows_IE_jmp
                           (<[PC:=WCap p b e a]> (<[idc:=widc]> regs))
-                          src p0 b0 e0 a0)) as [HallowJmp|_].
+                          src p0 b0 e0 a0) /\ cond_jmp)) as [HallowJmp|HallowJmp].
       { (* contradiction *)
         rewrite /reg_allows_IE_jmp in HallowJmp.
-        destruct HallowJmp as (Hregs0 & -> & Hwb & Hwb').
+        destruct HallowJmp as [(Hregs0 & -> & Hwb & Hwb') _].
         simplify_eq.
       }
       iModIntro.
-      iDestruct "HJmpMem" as "(_&->)". rewrite -memMap_resource_1.
+      iDestruct "HJmpMem" as "->". rewrite -memMap_resource_1.
       iMod ("Hcls" with "[Hmem HP]") as "_";[iExists w;iFrame|iModIntro].
       iApply wp_pure_step_later; auto.
 
@@ -553,8 +550,7 @@ Section fundamental.
           assert ( src <> PC ).
           { destruct (decide (src = PC)) ; simplify_map_eq ; destruct Hp; auto. }
           simplify_map_eq.
-          destruct (decide (src = idc)) ; simplify_map_eq; auto.
-          iApply "Hreg"; auto.
+          iApply "Hreg'"; auto.
           }
           rewrite (fixpoint_interp1_eq (WCap E _ _ _)) //=.
           rewrite (insert_commute _ PC _ (WCap RX _ _ _)) //=.
@@ -580,8 +576,7 @@ Section fundamental.
           clear Hsome' HVsrc HAJmpMem HAJmpReg.
 
           destruct (decide (src = PC)); simplify_map_eq; auto.
-          destruct (decide (src = idc)); simplify_map_eq; auto.
-          iApply "Hreg" ; auto.
+          iApply "Hreg'" ; auto.
         }
         { iFrame "Hinv_idc". }
       }
@@ -597,66 +592,30 @@ Section fundamental.
 
     - (* fail *)
       inversion Hfail as [? ? ? Hregs Hbounds ].
-      destruct (decide (reg_allows_IE_jmp
+      rewrite /allow_jmp_mask_reg /allow_jmp_mem /allow_jmp_res.
+      destruct (decide ((reg_allows_IE_jmp
                           (<[PC:=WCap p b e a]> (<[idc:=widc]> regs))
-                          src p0 b0 e0 a0)) as [HallowJmp|_]
+                          src p0 b0 e0 a0) /\ cond_jmp)) as [HallowJmp|_]
       ; cycle 1.
       {
         iModIntro.
-        iDestruct "HJmpMem" as "(_&->)". rewrite -memMap_resource_1.
+        iDestruct "HJmpMem" as "->". rewrite -memMap_resource_1.
         iMod ("Hcls" with "[Hmem HP]") as "_";[iExists w;iFrame|iModIntro].
         iApply wp_pure_step_later; auto.
         iNext; iIntros "_".
         iApply wp_value; auto; iIntros; discriminate.
       }
-      iDestruct "HJmpMem" as "(_&H)".
+
       assert ((a0 ^+ 1)%a ≠ a0) as Ha0eq
-      by (destruct HallowJmp as (_ & _ & Hwb%Is_true_true_1%withinBounds_true_iff & _); solve_addr).
+      by (destruct HallowJmp as
+           [(_ & _ & Hwb%Is_true_true_1%withinBounds_true_iff & _) _]; solve_addr).
+      assert (p0 = IE /\ b0 = b1 /\ e0 = e1 /\ a0 = a1) as (-> & <- & <- & <-)
+          by (by rewrite /read_reg_inr in HVsrc; rewrite Hregs in HVsrc; simplify_eq).
 
-      (* TODO duplicated proof... could be better *)
-      destruct (decide (a = a0)) as [Ha|Ha]; simplify_map_eq.
-      { (* a = a0 *)
-        iDestruct "H" as (w2) "(->&Hres)". rewrite /region_open_resources'.
-        rewrite memMap_resource_2ne; auto.
-        iDestruct "Hmem" as "(Ha0' & Ha0)".
-        iDestruct "Hres" as "(HP2 & _ & Hcls')".
-        rewrite /allow_jmp_mask.
-        case_decide as H'; simplify_eq.
-        iMod ("Hcls'" with "[HP2 Ha0']") as "_"
-        ; [iNext ; iExists w2; iFrame|iModIntro].
-        iMod ("Hcls" with "[Ha0 HP]") as "_";[iExists w;iFrame|iModIntro].
-        iApply wp_pure_step_later; auto.
-        iNext; iIntros "_".
-        iApply wp_value; auto; iIntros; discriminate.
-      }
-      (* a <> a0 *)
-      destruct (decide (a = (a0 ^+1)%a)) as [Ha'|Ha']; simplify_map_eq.
-      { (* a = a0+1 *)
-        iDestruct "H" as (w1) "(->&Hres)". rewrite /region_open_resources.
-        rewrite memMap_resource_2ne; auto.
-        iDestruct "Hmem" as "(Ha0 & Ha0')".
-        iDestruct "Hres" as "(HP1 & _ & Hcls')".
-        rewrite /allow_jmp_mask.
-        case_decide as H'; simplify_eq; clear H'.
-        case_decide as H'; simplify_eq.
-        iMod ("Hcls'" with "[HP1 Ha0]") as "_"
-        ; [iNext ; iExists w1; iFrame|iModIntro].
-        iMod ("Hcls" with "[Ha0' HP]") as "_";[iExists w;iFrame|iModIntro].
-        iApply wp_pure_step_later; auto.
-        iNext; iIntros "_".
-        iApply wp_value; auto; iIntros; discriminate.
-      }
+      (* Step 4: return all the resources we had *)
+      iMod (mem_map_recover_res with "HJmpMem Hmem") as "Ha"; auto.
 
-      (* a <> a0+1 *)
-      iDestruct "H" as (w1 w2) "(->&Hres)". rewrite /region_open_resources2.
-      rewrite memMap_resource_3ne; auto.
-      iDestruct "Hmem" as "(Ha0' & Ha0 & Ha)".
-      iDestruct "Hres" as "(HP1 & HP2 & _& _ & Hcls')".
-      rewrite /allow_jmp_mask.
-      case_decide as H'; simplify_eq ; clear H'.
-      case_decide as H'; simplify_eq ; clear H'.
-      iMod ("Hcls'" with "[HP1 HP2 Ha0 Ha0']") as "_"
-      ; [iNext ; iExists w1, w2; iFrame|iModIntro].
+      iModIntro.
       iMod ("Hcls" with "[Ha HP]") as "_";[iExists w;iFrame|iModIntro].
       iApply wp_pure_step_later; auto.
       iNext; iIntros "_".
