theories/ftlr/Jnz.v
@@ -2,8 +2,8 @@ From iris.proofmode Require Import proofmode.
 From iris.program_logic Require Import weakestpre adequacy lifting.
 From stdpp Require Import base.
 From cap_machine Require Export logrel register_tactics.
-From cap_machine.ftlr Require Import ftlr_base.
 From cap_machine.rules Require Import rules_Jnz.
+From cap_machine.ftlr Require Import ftlr_base Jmp.
 
 Section fundamental.
   Context {Σ:gFunctors} {memg:memG Σ} {regg:regG Σ} {sealsg: sealStoreG Σ}
@@ -15,388 +15,70 @@ Section fundamental.
   Implicit Types w : (leibnizO Word).
   Implicit Types interp : (D).
 
-
-  (* TODO the whole proof strategy is very similar to the one for Jmp.
-     Is there a way to factor out both of them ? *)
-
-  (* Mask after the jump, depending on the address of the pc and the address
-   of a *)
-  Definition allow_jnz_mask (pc_a a : Addr) : coPset
-    :=
-    if decide (pc_a = a)
-    then (⊤ ∖ ↑logN.@pc_a ∖ ↑logN.@(a^+1)%a)
-    else
-      if decide (pc_a = (a^+1)%a)
-      then (⊤ ∖ ↑logN.@pc_a ∖ ↑logN.@a)
-      else (⊤ ∖ ↑logN.@pc_a ∖ ↑logN.@a ∖ ↑logN.@(a^+1)%a).
-
-
-  Definition allow_jnz_mask_reg (regs : Reg) (dst src : RegName)
-    (pc_a : Addr) (p : Perm) (b e a : Addr) (wsrc : Word)
-    : coPset :=
-    if decide (reg_allows_IE_jmp regs dst p b e a
-               /\ regs !! src = Some wsrc
-               /\ nonZero wsrc = true)
-    then allow_jnz_mask pc_a a
-    else (⊤ ∖ ↑logN.@pc_a).
-
-  (* The necessary resources to close the region again,
-     except for the points to predicate, which we will store separately *)
-  Definition region_open_resources2
-    (pc_a : Addr) (a : Addr)
-    (w1 : Word) (w2 : Word)
-    (P1 P2 : D)
-    : iProp Σ :=
-    ▷ P1 w1 ∗ ▷ P2 w2
-       ∗ persistent_cond P1 ∗ persistent_cond P2
-       ∗ ((▷ ∃ w1 w2, a ↦ₐ w1 ∗ P1 w1 ∗ (a^+1)%a ↦ₐ w2 ∗ P2 w2)
-          ={allow_jnz_mask pc_a a, ⊤ ∖ ↑logN.@pc_a}=∗ emp)%I.
-
-  Definition region_open_resources
-    (pc_a : Addr) (a : Addr) (w : Word)
-    (P : D)
-    : iProp Σ :=
-    (▷ P w
-       ∗ persistent_cond P
-       ∗ ((▷ ∃ w, a ↦ₐ w ∗ P w)
-        ={allow_jnz_mask pc_a a, ⊤ ∖ ↑logN.@pc_a}=∗ emp))%I.
-
-  Definition region_open_resources'
-    (pc_a : Addr) (a : Addr) (w' : Word)
-    (P : D)
-    : iProp Σ :=
-    (▷ P w'
-       ∗ persistent_cond P
-       ∗ ((▷ ∃ w', (a^+1)%a ↦ₐ w' ∗ P w')
-        ={allow_jnz_mask pc_a a, ⊤ ∖ ↑logN.@pc_a}=∗ emp))%I.
-
-  (* Description of what the resources are supposed to look like after opening the
-     region if we need to, but before closing the region up again*)
-  Definition allow_jnz_res (regs : Reg) (dst src : RegName)
-    (pc_a : Addr) (p : Perm) (b e a : Addr) (wsrc : Word)
-    (P1 P2 : D): iProp Σ :=
-    ( ⌜read_reg_inr regs dst p b e a⌝ ∗
-      ⌜regs !! src = Some wsrc⌝ ∗
-       if decide (reg_allows_IE_jmp regs dst p b e a
-               /\ regs !! src = Some wsrc
-               /\ nonZero wsrc = true)
-       then
-         (∀ w1 w2 regs', ▷ □ (P1 w1 ∗ (P2 w2 ∨ ⌜ is_int w2 ⌝)
-                              -∗ (interp_expr_gen interp regs' w1 w2)))
-           ∗
-           |={⊤ ∖ ↑logN.@pc_a, allow_jnz_mask pc_a a}=>
-           (if decide (pc_a = a)
-            then ∃ w2, (a^+1)%a ↦ₐ w2 ∗ region_open_resources' pc_a a w2 P2
-            else
-              if decide (pc_a = (a^+1)%a)
-              then ∃ w1, a ↦ₐ w1 ∗ region_open_resources pc_a a w1 P1
-              else ∃ w1 w2, a ↦ₐ w1 ∗ (a^+1)%a ↦ₐ w2 ∗ region_open_resources2 pc_a a w1 w2 P1 P2
-           )
-       else True)%I.
-
-  Lemma create_jnz_res:
-    ∀ (regs : leibnizO Reg) (dst src : RegName)
-      (pc_p : Perm) (pc_b pc_e pc_a : Addr)
-      (widc : Word)
-      (p : Perm) (b e a : Addr) (wsrc : Word),
-      pc_p <> IE ->
-      read_reg_inr (<[PC:=WCap pc_p pc_b pc_e pc_a]> (<[idc:= widc]> regs)) dst p b e a ->
-      (<[PC:=WCap pc_p pc_b pc_e pc_a]> (<[idc:= widc]> regs)) !! src = Some wsrc ->
-      (∀ (r' : RegName) (w : Word), ⌜r' ≠ PC⌝ → ⌜r' ≠ idc⌝ → ⌜regs !! r' = Some w⌝ → (fixpoint interp1) w)
-      -∗ interp widc
-      -∗ ∃ (P1 P2 : D),
-           allow_jnz_res (<[PC:=WCap pc_p pc_b pc_e pc_a]> (<[idc:=widc]> regs)) dst src pc_a p b
-             e a wsrc P1 P2.
-  Proof.
-    intros regs dst src pc_p pc_b pc_e pc_a widc p b e a wsrc Hpc_p HVr Hsrc.
-    iIntros "#Hreg #Hwidc".
-    iFrame "%".
-    case_decide as Hallows; cycle 1.
-    - by iExists (λne _, True%I), (λne _, True%I).
-    - rewrite /allow_jnz_mask.
-      destruct Hallows as ((Hreg & -> & Hwb & Hwb') & Hsrc' & Hnz).
-      assert (a <> (a^+1)%a) by (apply Is_true_true_1, andb_prop in Hwb as [_ Hge]; solve_addr).
-      assert ( withinBounds b e a /\ withinBounds b e (a^+1)%a) as Hwbs by auto.
-
-      assert (dst ≠ PC) as Hneq by (destruct (decide (dst = PC)) ; simplify_map_eq; auto).
-      rewrite lookup_insert_ne //= in Hreg.
-
-      (* TODO there are plenty of similar case, find a way to factor out *)
-
-      case_decide as Ha; simplify_eq.
-      {
-        destruct (decide (dst = idc)) as [|Hneq']; simplify_map_eq.
-        + rewrite fixpoint_interp1_eq /=.
-          iDestruct ("Hwidc" $! Hwbs) as (P1 P2) "(Hpers_P1 & Hpers_P2 & Hinv_a & Hinv_a' & Hexec)".
-          iExists P1, P2.
-          iFrame "#".
-          iMod (inv_acc (⊤ ∖ ↑logN.@a) with "Hinv_a'") as "[Hrefinv_a' Hcls_a']";[solve_ndisj|].
-          iDestruct "Hrefinv_a'" as (w2) "[>Ha' HPa']".
-          iExists w2.
-          iFrame "∗ #".
-          rewrite /allow_jnz_mask. do 2 (case_decide ; solve_addr).
-        + iDestruct ("Hreg" $! dst _ Hneq Hneq' Hreg) as "Hvsrc".
-          rewrite (fixpoint_interp1_eq (WCap _ _ _ _)) /=.
-          iDestruct ("Hvsrc" $! Hwbs) as (P1 P2) "(Hpers_P1 & Hpers_P2 & Hinv_a & Hinv_a' & Hexec)".
-          iExists P1, P2.
-          iFrame "#".
-          iMod (inv_acc (⊤ ∖ ↑logN.@a) with "Hinv_a'") as "[Hrefinv_a' Hcls_a']";[solve_ndisj|].
-          iDestruct "Hrefinv_a'" as (w2) "[>Ha' HPa']".
-          iExists w2.
-          iFrame "∗ #".
-          rewrite /allow_jnz_mask. do 2 (case_decide ; solve_addr).
-      }
-
-      case_decide as Ha'; simplify_eq.
-      {
-        destruct (decide (dst = idc)) as [|Hneq']; simplify_map_eq.
-        + rewrite fixpoint_interp1_eq /=.
-          iDestruct ("Hwidc" $! Hwbs) as (P1 P2) "(Hpers_P1 & Hpers_P2 & Hinv_a & Hinv_a' & Hexec)".
-          iExists P1, P2.
-          iFrame "#".
-          iMod (inv_acc (⊤ ∖ ↑logN.@(a ^+ 1)%a) with "Hinv_a") as "[Hrefinv_a Hcls_a]";[solve_ndisj|].
-          iDestruct "Hrefinv_a" as (w1) "[>Ha HPa]".
-          iExists w1.
-          iFrame "∗ #".
-          rewrite /allow_jnz_mask. do 2 (case_decide ; try solve_addr).
-        + iDestruct ("Hreg" $! dst _ Hneq Hneq' Hreg) as "Hvsrc".
-          rewrite (fixpoint_interp1_eq (WCap _ _ _ _)) /=.
-          iDestruct ("Hvsrc" $! Hwbs) as (P1 P2) "(Hpers_P1 & Hpers_P2 & Hinv_a & Hinv_a' & Hexec)".
-          iExists P1, P2.
-          iFrame "#".
-          iMod (inv_acc (⊤ ∖ ↑logN.@(a ^+ 1)%a) with "Hinv_a") as "[Hrefinv_a Hcls_a]";[solve_ndisj|].
-          iDestruct "Hrefinv_a" as (w1) "[>Ha HPa]".
-          iExists w1.
-          iFrame "∗ #".
-          rewrite /allow_jnz_mask. do 2 (case_decide ; try solve_addr).
-      }
-
-      destruct (decide (dst = idc)) as [|Hneq']; simplify_map_eq.
-      + rewrite fixpoint_interp1_eq /=.
-        iDestruct ("Hwidc" $! Hwbs) as (P1 P2) "(Hpers_P1 & Hpers_P2 & Hinv_a & Hinv_a' & Hexec)".
-        iExists P1, P2.
-
-        iFrame "#".
-        iMod (inv_acc (⊤ ∖ ↑logN.@pc_a) with "Hinv_a") as "[Hrefinv_a Hcls_a]";[solve_ndisj|].
-        iMod (inv_acc (⊤ ∖ ↑logN.@pc_a ∖ ↑logN.@a) with "Hinv_a'") as "[Hrefinv_a' Hcls_a']";[solve_ndisj|].
-        iDestruct "Hrefinv_a" as (w1) "[>Ha HPa]".
-        iDestruct "Hrefinv_a'" as (w2) "[>Ha' HPa']".
-        iExists w1, w2.
-
-        iFrame "∗ #".
-        rewrite /region_open_resources2.
-        iModIntro.
-        iIntros "Ha".
-        iDestruct "Ha" as (w1' w2') "(Hw1' & HP1' & Hw2' & HP2')".
-        rewrite /allow_jnz_mask.
-        case_decide; simplify_eq.
-        case_decide; simplify_eq.
-        iMod ("Hcls_a'" with "[Hw2' HP2']") as "_"; first (iExists _ ; iFrame).
-        iMod ("Hcls_a" with "[Hw1' HP1']") as "_"; first (iExists _ ; iFrame).
-        done.
-      + iDestruct ("Hreg" $! dst _ Hneq Hneq' Hreg) as "Hvsrc".
-        rewrite (fixpoint_interp1_eq (WCap _ _ _ _)) /=.
-        iDestruct ("Hvsrc" $! Hwbs) as (P1 P2) "(Hpers_P1 & Hpers_P2 & Hinv_a & Hinv_a' & Hexec)".
-        iExists P1, P2.
-
-        iFrame "#".
-        iMod (inv_acc (⊤ ∖ ↑logN.@pc_a) with "Hinv_a") as "[Hrefinv_a Hcls_a]";[solve_ndisj|].
-        iMod (inv_acc (⊤ ∖ ↑logN.@pc_a ∖ ↑logN.@a) with "Hinv_a'") as "[Hrefinv_a' Hcls_a']";[solve_ndisj|].
-        iDestruct "Hrefinv_a" as (w1) "[>Ha HPa]".
-        iDestruct "Hrefinv_a'" as (w2) "[>Ha' HPa']".
-        iExists w1, w2.
-
-        iFrame "∗ #".
-        rewrite /region_open_resources2.
-        iModIntro.
-        iIntros "Ha".
-        iDestruct "Ha" as (w1' w2') "(Hw1' & HP1' & Hw2' & HP2')".
-        rewrite /allow_jnz_mask.
-        case_decide; simplify_eq.
-        case_decide; simplify_eq.
-        iMod ("Hcls_a'" with "[Hw2' HP2']") as "_"; first (iExists _ ; iFrame).
-        iMod ("Hcls_a" with "[Hw1' HP1']") as "_"; first (iExists _ ; iFrame).
-        done.
-  Qed.
-
-  Definition allow_jnz_mem
-    (regs : Reg) (mem : Mem) (dst src : RegName)
-    (pc_a : Addr) (pc_w : Word)
-    (p : Perm) (b e a : Addr) (wsrc : Word)
-    (P1 P2 : D) :=
-    ( ⌜read_reg_inr regs dst p b e a⌝ ∗
-      ⌜regs !! src = Some wsrc⌝ ∗
-       if decide (reg_allows_IE_jmp regs dst p b e a
-               /\ regs !! src = Some wsrc
-               /\ nonZero wsrc = true)
-       then (if decide (pc_a = a)
-             then ∃ w2, ⌜mem = <[(a^+1)%a:=w2]> (<[pc_a:=pc_w]> ∅)⌝ ∗ region_open_resources' pc_a a w2 P2
-             else
-               if decide (pc_a = (a^+1)%a)
-               then ∃ w1, ⌜mem = <[a:=w1]> (<[pc_a:=pc_w]> ∅)⌝ ∗ region_open_resources pc_a a w1 P1
-               else ∃ w1 w2,
-                   ⌜mem = <[(a^+1)%a:=w2]> (<[a:=w1]> (<[pc_a:=pc_w]> ∅))⌝
-                                             ∗ region_open_resources2 pc_a a w1 w2 P1 P2)
-       else ⌜mem = <[pc_a:=pc_w]> ∅⌝)%I.
-
-  Lemma jnz_res_implies_mem_map:
-    ∀ (regs : leibnizO Reg) (dst src: RegName)
-      (pc_a : Addr) (pc_w : Word)
-      (p : Perm) (b e a: Addr) (wsrc : Word)
-      (P1 P2:D),
-      allow_jnz_res regs dst src pc_a p b e a wsrc P1 P2
-      -∗ pc_a ↦ₐ pc_w
-      ={⊤ ∖ ↑logN.@pc_a, allow_jnz_mask_reg regs dst src pc_a p b e a wsrc}=∗
-      ∃ mem : Mem,
-          allow_jnz_mem regs mem dst src pc_a pc_w p b e a wsrc P1 P2
-            ∗ ▷ ([∗ map] a0↦w ∈ mem, a0 ↦ₐ w).
-  Proof.
-    intros regs dst src pc_a pc_w p b e a wsrc P1 P2.
-    iIntros "HJmpRes Hpc_a".
-    iDestruct "HJmpRes" as "(%Hrinr & %Hsrc & HJmpRes)".
-    rewrite /allow_jnz_mask /allow_jnz_mask_reg.
-
-    case_decide as Hdec ; cycle 1.
-    { rewrite /read_reg_inr in Hrinr.
-      iExists _.
-      iSplitL "HJmpRes".
-      + iModIntro. rewrite /allow_jnz_mem.
-        do 2 (iSplitR; auto).
-        case_decide; auto; first by exfalso.
-      + iModIntro. iNext. by iApply memMap_resource_1.
-    }
-    destruct Hdec as ((Hreg & -> & Hwb & Hwb') & Hsrc' & Hnz).
-    assert (a <> (a^+1)%a) as Haeq by (apply Is_true_true_1,andb_prop in Hwb as [_ Hge]; solve_addr).
-    rewrite /allow_jnz_mask.
-    iDestruct "HJmpRes" as "[Hexec HJmpRes]".
-    iMod "HJmpRes" as "HJmpRes".
-
-    case_decide as Ha ; simplify_eq.
-    { (* pc_a = a *)
-      iDestruct "HJmpRes" as (w2) "[Ha' HJmpRest]".
-      iExists _.
-      iSplitL "HJmpRest".
-      + iSplitR; first auto.
-
-        case_decide as Hdec1.
-        2: {
-          apply not_and_r in Hdec1 as [Hcontra|Hcontra]; simplify_eq.
-          all: exfalso; apply Hcontra ; repeat (split ; auto).
-        }
-        case_decide; simplify_eq; auto.
-      + iModIntro. iNext.
-        rewrite memMap_resource_2ne; auto; iFrame.
-    }
-    (* pc_a ≠ a *)
-    case_decide as Ha' ; simplify_eq.
-    { (* pc_a = a+1 *)
-      iDestruct "HJmpRes" as (w1) "[Ha HJmpRest]".
-      iExists _.
-      iSplitL "HJmpRest".
-      + iSplitR; first auto.
-        case_decide as Hdec1.
-        2: {
-          apply not_and_r in Hdec1 as [Hcontra|Hcontra]; simplify_eq.
-          all: exfalso; apply Hcontra ; repeat (split ; auto).
-        }
-        case_decide; simplify_eq; auto.
-        case_decide; simplify_eq; auto.
-      + iModIntro. iNext.
-        rewrite memMap_resource_2ne; auto; iFrame.
-    }
-    (* pc_a ≠ a+1 *)
-
-    iDestruct "HJmpRes" as (w1 w2) "(Ha & Ha' & HJmpRest)".
-    iExists _.
-    iSplitL "HJmpRest".
-    + iSplitR; first auto.
-      case_decide as Hdec1.
-      2: {
-        apply not_and_r in Hdec1 as [Hcontra|Hcontra]; simplify_eq.
-        all: exfalso; apply Hcontra ; repeat (split ; auto).
-      }
-      case_decide; simplify_eq; auto.
-      case_decide; simplify_eq; auto.
-      iModIntro; auto.
-    + iModIntro. iNext.
-      rewrite memMap_resource_3ne; auto; iFrame.
-  Qed.
-
+  (* Derice pure conds =allow_jnz_mmap_or_true= from =cond_jnz= *)
   Lemma mem_map_implies_pure_conds:
-    ∀ (regs : leibnizO Reg) (mem : Mem) (dst src : RegName)
+    ∀ (regs : Reg) (mem : Mem) (dst src : RegName)
       (pc_a : Addr) (pc_w : Word)
       (p : Perm) (b e a : Addr) (wsrc : Word)
       (P1 P2 : D),
-      allow_jnz_mem regs mem dst src pc_a pc_w p b e a wsrc P1 P2
+      read_reg_inr regs dst p b e a
+      -> regs !! src = Some wsrc
+      -> allow_jmp_mem (cond_jnz regs src wsrc) regs mem dst pc_a pc_w p b e a P1 P2
         -∗ ⌜mem !! pc_a = Some pc_w⌝
-          ∗ ⌜allow_jnz_mmap_or_true dst src regs mem⌝.
+          ∗ ⌜allow_jmp_mmap_or_true (cond_jnz regs src wsrc) dst regs mem⌝.
   Proof.
-    iIntros (regs mem dst src pc_a pc_w p b e a wsrc P1 P2) "HJmpMem".
-    iDestruct "HJmpMem" as "(%Hrinr & %Hsrc & HJmpRes)".
+    iIntros (regs mem dst src pc_a pc_w p b e a wsrc P1 P2 Hrinr Hsrc) "HJmpMem".
+    rewrite /allow_jmp_mem.
     case_decide as Hdec ; cycle 1.
-    { iDestruct "HJmpRes" as "->".
+    { iDestruct "HJmpMem" as "->".
       iSplitR. by rewrite lookup_insert.
-      iPureIntro ; intros ? ? Hnz.
+      iPureIntro.
       exists p,b,e,a.
       split; auto.
-      apply not_and_r in Hdec as [Hcontra|Hcontra]; simplify_eq; cycle 1.
-      apply not_and_r in Hcontra as [Hcontra|Hcontra]; simplify_eq.
-      apply Is_true_true_1 in Hnz.
-      done.
-      by destruct (decide (reg_allows_IE_jmp regs dst p b e a)).
+      rewrite decide_False //=.
     }
-    destruct Hdec as (Hdec & _ & Hnz).
+    destruct Hdec as (Hdec & Hjnz).
+
+    rewrite /allow_jmp_mem_res.
     assert (a <> (a^+1)%a)
     by (inversion Hdec as (_ & _ & Hwb%Is_true_true_1%withinBounds_true_iff & _); solve_addr).
+
     case_decide as Ha; simplify_eq.
-    { iDestruct "HJmpRes" as (w2) "[%Hmem _]" ; subst.
+    { (* pc_a = a *)
+      iDestruct "HJmpMem" as (w2) "[%Hmem _]" ; subst.
       iSplitL; iPureIntro.
       by simplify_map_eq.
-      intros ? ? ?. exists p,b,e,a.
+      exists p,b,e,a.
       split;auto.
-      simplify_eq.
-      case_decide; auto.
-      inversion Hdec.
+      rewrite decide_True //=.
       exists pc_w, w2.
       by split ; simplify_map_eq.
     }
+
     case_decide as Ha'; simplify_eq.
-    { iDestruct "HJmpRes" as (w1) "[%Hmem _]" ; subst.
+    { (* pc_a = a+1 *)
+      iDestruct "HJmpMem" as (w1) "[%Hmem _]" ; subst.
       iSplitL; iPureIntro.
       by simplify_map_eq.
-      intros ? ? ?. exists p,b,e,a.
+      exists p,b,e,a.
       split;auto.
-      simplify_eq.
-      case_decide; auto.
-      inversion Hdec.
+      rewrite decide_True //=.
       exists w1, pc_w.
       by split ; simplify_map_eq.
     }
 
-    iDestruct "HJmpRes" as (w1 w2) "[%Hmem _]" ; subst.
+    (* pc_a ≠ a ∧ pc_a ≠ a+1 *)
+    iDestruct "HJmpMem" as (w1 w2) "[%Hmem _]" ; subst.
     iSplitL; iPureIntro.
     by simplify_map_eq.
-    intros ? ? ?. exists p,b,e,a.
+    exists p,b,e,a.
     split;auto.
-    simplify_eq.
-    case_decide; auto.
+    rewrite decide_True //=.
     exists w1, w2.
     by split ; simplify_map_eq.
   Qed.
 
-  Lemma reg_allows_IE_jmp_same
-    (regs : Reg) (r : RegName)
-    (p p' : Perm) (b b' e e' a a' : Addr):
-    reg_allows_IE_jmp regs r p b e a ->
-    regs !! r = Some (WCap p' b' e' a') ->
-    (p = p' /\ b = b' /\ e = e' /\ a = a').
-  Proof.
-    intros HallowJmp Hregs.
-    destruct HallowJmp as (Hregs'&->&_).
-    by rewrite Hregs' in Hregs; simplify_eq.
-  Qed.
-
-  Lemma jnz_case (regs : leibnizO Reg) (p : Perm)
+  Lemma jnz_case (regs : Reg) (p : Perm)
         (b e a : Addr) (widc w : Word) (dst src : RegName) (P : D):
     ftlr_instr regs p b e a widc w (Jnz dst src) P.
   Proof.
@@ -434,213 +116,179 @@ Section fundamental.
       by eexists.
     }
 
+    iAssert (
+        ∀ (r' : RegName) (w : Word),
+          ⌜r' ≠ PC⌝ → ⌜<[idc:=widc]> regs  !! r' = Some w⌝ → fixpoint interp1 w
+      )%I as "Hreg'".
+    { iIntros.
+      destruct (decide (r' = idc)); simplify_map_eq; auto.
+      iApply "Hreg";eauto.
+    }
+
+    set (Hcond_jnz := cond_jnz (<[PC:=WCap p b e a]> (<[idc:=widc]> regs)) src wsrc).
+
     (* Step 1: open the region, if necessary, and store all the resources
        obtained from the region in allow_IE_res *)
-    iDestruct (create_jnz_res with "Hreg Hinv_idc") as (P1 P2) "HJmpRes"; eauto.
+    iDestruct ((create_jmp_res Hcond_jnz _ _ p)  with "Hreg'") as (P1 P2) "HJmpRes"; eauto.
     { destruct Hp ; destruct p ; auto. }
 
     (* Step2: derive the concrete map of memory we need, and any spatial
        predicates holding over it *)
-    iMod (jnz_res_implies_mem_map with "HJmpRes Ha") as (mem) "[HJmpMem HJmpRest]".
+    iMod ((jmp_res_implies_mem_map Hcond_jnz)
+           with "HJmpRes Ha") as (mem) "[HJmpMem HJmpRest]"; eauto.
 
     (* Step 3:  derive the non-spatial conditions over the memory map*)
-    iDestruct (mem_map_implies_pure_conds with "HJmpMem") as
-      %(HReadPC & HAJmpMem); auto.
+    iDestruct ((mem_map_implies_pure_conds _ mem dst src a w p0 b0 e0 a0 wsrc P1 P2)
+                with "HJmpMem") as %(HReadPC & HAJmpMem); eauto.
 
     (* Step 3.5:  derive the non-spatial conditions over the registers *)
-    iAssert (⌜allow_jnz_rmap_or_true dst src
-               (<[PC:=WCap p b e a]> (<[idc:=widc]> regs))⌝)%I as "%HAJmpReg".
-    { rewrite /allow_jnz_rmap_or_true.
-      iIntros (wsrc0) "%Hsrc0 %Hnz0".
-      iExists p0, b0, e0, a0.
-      iSplit; auto.
-      case_decide as Heq; auto.
-      by iExists widc; simplify_map_eq.
+    assert (allow_jmp_rmap_or_true Hcond_jnz dst (<[PC:=WCap p b e a]> (<[idc:=widc]> regs)))
+      as HAJmpReg.
+    { rewrite /allow_jmp_rmap_or_true.
+      exists p0, b0, e0, a0.
+      split; auto.
+      (* TODO any way to avoid manual match ? *)
+      match goal with
+      | H: _ |- (if (decide ?cond) then _ else _) =>
+          destruct (decide cond)
+      end; auto.
+      by eexists _; simplify_map_eq.
     }
 
+    assert (
+        regs_of (Jnz dst src) ⊆ dom (<[PC:=WCap p b e a]> (<[idc:=widc]> regs))
+      ).
+    { rewrite /subseteq /map_subseteq /set_subseteq_instance. intros rr _.
+      apply elem_of_dom. repeat (rewrite lookup_insert_is_Some'; right); eauto. }
     iApply (wp_Jnz _ _ _ _ _ _ _ _ (<[PC:=WCap p b e a]> (<[idc:=widc]> regs))
              with "[Hmap HJmpRest]");eauto.
     { by simplify_map_eq. }
-    { rewrite /subseteq /map_subseteq /set_subseteq_instance. intros rr _.
-      apply elem_of_dom. repeat (rewrite lookup_insert_is_Some'; right); eauto. }
     { iSplitR "Hmap"; auto. }
     iNext. iIntros (regs' retv). iDestruct 1 as (HSpec) "[Hmem Hmap]".
     (* Infer that if P holds at w, then w must be valid (read condition) *)
     iDestruct ("Hread" with "HP") as "#Hw".
-    rewrite /allow_jnz_res /allow_jnz_mem /allow_jnz_mask_reg /allow_jnz_mask.
+    rewrite /allow_jmp_res /allow_jmp_mem /allow_jmp_mask_reg /allow_jmp_mask.
 
     destruct HSpec as
       [ Hfail
-      | * Hsrc Hdst Hcond Hwb Hwb' Ha Ha' HincrPC (* Success IE true*)
+      | * Hsrc Hdst Hcond Hwb Hwb' Ha Ha' HincrPC (* Success IE true *)
       | * Hsrc Hdst Hcond HnIE HincrPC (* Success true *)
       | * Hsrc Hcond HincrPC (* Success false *)
       ].
     - (* Fail *)
-      case_decide as HallowJmp; cycle 1.
+      match goal with
+      | H: _ |- context [(if (decide ?cond) then _ else _)] =>
+          destruct (decide cond) as [HallowJmp|HallowJmp] ; cycle 1
+      end; auto.
       {
         iModIntro.
-        iDestruct "HJmpMem" as "(_&_&->)". rewrite -memMap_resource_1.
+        iDestruct "HJmpMem" as "->". rewrite -memMap_resource_1.
         iMod ("Hcls" with "[Hmem HP]") as "_";[iExists w;iFrame|iModIntro].
         iApply wp_pure_step_later; auto.
         iNext; iIntros "_".
         iApply wp_value; auto; iIntros; discriminate.
       }
-      iDestruct "HJmpMem" as "(_&_&H)".
-      destruct HallowJmp as (HallowJmp & _ & Hnz).
+      destruct HallowJmp as (HallowJmp & _).
       assert ((a0 ^+ 1)%a ≠ a0) as Ha0eq
           by (destruct HallowJmp as (_ & _ & Hwb%Is_true_true_1%withinBounds_true_iff & _); solve_addr).
+      rewrite /allow_jmp_mem_res /allow_jmp_mask.
 
-      (* TODO duplicated proof... could be better *)
-      destruct (decide (a = a0)) as [Ha|Ha]; simplify_map_eq.
-      { (* a = a0 *)
-        iDestruct "H" as (w2) "(->&Hres)". rewrite /region_open_resources'.
-        rewrite memMap_resource_2ne; auto.
-        iDestruct "Hmem" as "(Ha0' & Ha0)".
-        iDestruct "Hres" as "(HP2 & _ & Hcls')".
-        rewrite /allow_jnz_mask.
-        case_decide as H'; simplify_eq.
-        iMod ("Hcls'" with "[HP2 Ha0']") as "_"
-        ; [iNext ; iExists w2; iFrame|iModIntro].
-        iMod ("Hcls" with "[Ha0 HP]") as "_";[iExists w;iFrame|iModIntro].
-        iApply wp_pure_step_later; auto.
-        iNext; iIntros "_".
-        iApply wp_value; auto; iIntros; discriminate.
-      }
-      (* a <> a0 *)
-      destruct (decide (a = (a0 ^+1)%a)) as [Ha'|Ha']; simplify_map_eq.
-      { (* a = a0+1 *)
-        iDestruct "H" as (w1) "(->&Hres)". rewrite /region_open_resources.
-        rewrite memMap_resource_2ne; auto.
-        iDestruct "Hmem" as "(Ha0 & Ha0')".
-        iDestruct "Hres" as "(HP1 & _ & Hcls')".
-        rewrite /allow_jnz_mask.
-        case_decide as H'; simplify_eq; clear H'.
-        case_decide as H'; simplify_eq.
-        iMod ("Hcls'" with "[HP1 Ha0]") as "_"
-        ; [iNext ; iExists w1; iFrame|iModIntro].
-        iMod ("Hcls" with "[Ha0' HP]") as "_";[iExists w;iFrame|iModIntro].
-        iApply wp_pure_step_later; auto.
-        iNext; iIntros "_".
-        iApply wp_value; auto; iIntros; discriminate.
-      }
+      (* Step 4: return all the resources we had *)
+      iMod (mem_map_recover_res with "HJmpMem Hmem") as "Ha"; auto.
 
-      (* a <> a0+1 *)
-      iDestruct "H" as (w1 w2) "(->&Hres)". rewrite /region_open_resources2.
-      rewrite memMap_resource_3ne; auto.
-      iDestruct "Hmem" as "(Ha0' & Ha0 & Ha)".
-      iDestruct "Hres" as "(HP1 & HP2 & _& _ & Hcls')".
-      rewrite /allow_jnz_mask.
-      case_decide as H'; simplify_eq ; clear H'.
-      case_decide as H'; simplify_eq ; clear H'.
-      iMod ("Hcls'" with "[HP1 HP2 Ha0 Ha0']") as "_"
-      ; [iNext ; iExists w1, w2; iFrame|iModIntro].
+      iModIntro.
       iMod ("Hcls" with "[Ha HP]") as "_";[iExists w;iFrame|iModIntro].
       iApply wp_pure_step_later; auto.
       iNext; iIntros "_".
       iApply wp_value; auto; iIntros; discriminate.
 
-
     - (* Success IE true*)
       rewrite insert_insert insert_commute //= insert_insert in HincrPC; subst regs'.
-      case_decide as HallowJmp.
+      match goal with
+      | H: _ |- context [(if (decide ?cond) then _ else _)] =>
+          destruct (decide cond) as [HallowJmp|HallowJmp]
+      end; auto.
       2: { (* contradiction *)
         rewrite /reg_allows_IE_jmp in HallowJmp.
         rewrite /read_reg_inr in HVdst.
         rewrite Hdst in HVdst; simplify_eq.
-        rewrite Hsrc in HVsrc; simplify_eq.
         repeat (apply not_and_r in HallowJmp as [HallowJmp|HallowJmp] ; simplify_eq)
-        ; congruence.
+        ; try congruence.
+        exfalso. apply HallowJmp.
+        by rewrite /Hcond_jnz /cond_jnz; intros _.
       }
-      destruct HallowJmp as (HallowJmp & _ & Hnz).
+      destruct HallowJmp as (HallowJmp & _).
       assert (PC <> dst) as Hdst'
           by (destruct (decide (PC = dst)); auto; simplify_map_eq; by destruct Hp).
-      assert (p0 = IE /\ b0 = b1 /\ e0 = e1 /\ a0 = a1) as (-> & -> & -> & ->)
+      assert (p0 = IE /\ b0 = b1 /\ e0 = e1 /\ a0 = a1) as (-> & <- & <- & <-)
           by (by eapply reg_allows_IE_jmp_same)
       ; simplify_map_eq.
-      assert ((a1 ^+ 1)%a ≠ a1) as Haeq by (apply Is_true_true_1, withinBounds_true_iff in Hwb ; solve_addr).
-      assert (withinBounds b1 e1 a1 ∧ withinBounds b1 e1 (a1 ^+ 1)%a) as Hbounds by auto.
+      assert ((a0 ^+ 1)%a ≠ a0) as Haeq by (apply Is_true_true_1, withinBounds_true_iff in Hwb ; solve_addr).
+      assert (withinBounds b0 e0 a0 ∧ withinBounds b0 e0 (a0 ^+ 1)%a) as Hbounds
+          by auto.
 
-      iDestruct "HJmpMem" as "(_& %H' & HJmpMem)"; simplify_eq.
-      iDestruct "HJmpRes" as "(_& _ & Hexec &HJmpRes)".
-      case_decide as Ha0; simplify_eq.
+      iDestruct "HJmpRes" as "(Hexec&HJmpRes)".
+
+      (* Step 4: return all the resources we had *)
+      iMod ((mem_map_recover_res_ie _ _ _ w wpc widc0 P P1 P2) with "HJmpMem Hmem") as "Ha"
+      ; auto; iModIntro.
+
+
+      destruct_decide (decide (a = a0)) as Ha0; simplify_eq.
       { (* a = a0 *)
 
-        iDestruct "HJmpMem" as (w2) "(->& HP2& %Hpers2& Hcls')".
-        iDestruct "HP2" as "#HP2".
-        rewrite /allow_jnz_mask.
-        case_decide ; simplify_eq.
-        rewrite memMap_resource_2ne; auto.
-        simplify_map_eq.
+        iDestruct "Ha" as "[Ha0 ->]".
 
-        iDestruct "Hmem" as  "[Ha0' Ha0]".
-        iMod ("Hcls'" with "[HP2 Ha0']") as "_"; [iNext;iExists widc0;iFrame "∗ #"|iModIntro].
         iMod ("Hcls" with "[HP Ha0]") as "_"; [iNext;iExists wpc;iFrame|iModIntro].
         iClear "HJmpRes".
         iApply wp_pure_step_later; auto.
         iNext ; iIntros "_".
         destruct wpc; cbn in Hi; try done.
         iExtract "Hmap" PC as "HPC".
-
         iApply interp_expr_invalid_pc; try iFrame ; eauto.
         intro Hcontra; inversion Hcontra.
         iPureIntro; apply regmap_full_dom in Hsome; rewrite -Hsome; set_solver.
       }
 
-      (* a ≠ a0 *)
-      case_decide as Ha0'; simplify_eq.
+      destruct_decide (decide (a = (a0 ^+ 1)%a)) as Ha0'; simplify_eq.
       { (* a = a0+1 *)
 
-        iDestruct "HJmpMem" as (w1) "(->& HP1& %Hpers1& Hcls')".
+        iDestruct "Ha" as "(Ha0 & -> & HP1 & %Hpers1)".
         iDestruct "HP1" as "#HP1".
-        rewrite /allow_jnz_mask.
-        case_decide ; simplify_eq.
-        case_decide ; simplify_eq.
-        rewrite memMap_resource_2ne; auto.
-        simplify_map_eq.
 
-        iDestruct "Hmem" as  "[Ha0' Ha0]".
-        iMod ("Hcls'" with "[HP1 Ha0']") as "_"; [iNext;iExists wpc;iFrame "∗ #"|iModIntro].
         iMod ("Hcls" with "[HP Ha0]") as "_"; [iNext;iExists widc0;iFrame|iModIntro].
-        iClear "HJmpRes".
         iApply wp_pure_step_later; auto.
         iNext ; iIntros "_".
-
         iApply ("Hexec" $! _ widc0) ; iFrame "∗ #".
         iRight; destruct widc0; cbn in Hi; try done.
-
         rewrite insert_commute //=.
         repeat (iSplit ; try done).
       }
 
-      (* a ≠ a0+1 *)
-      iDestruct "HJmpMem" as (w1 w2) "(->& HP1& HP2& %Hpers1& %Hpers2& Hcls')".
-      rewrite /region_open_resources2.
+      (* a ≠ a0 ∧ a ≠ a0+1 *)
+      iDestruct "Ha" as "(Ha & HP1 & HP2 & %Hpers1 & %Hpers2)".
       iDestruct "HP1" as "#HP1"; iDestruct "HP2" as "#HP2".
-      rewrite /allow_jnz_mask; case_decide ; simplify_eq; case_decide ; simplify_eq.
-      rewrite memMap_resource_3ne; auto.
-      simplify_map_eq.
-
-      iDestruct "Hmem" as  "(Ha0' & Ha0 & Ha)".
-      iMod ("Hcls'" with "[HP1 HP2 Ha0' Ha0]") as "_"; [iNext;iExists wpc,widc0;iFrame "∗ #"|iModIntro].
       iMod ("Hcls" with "[HP Ha]") as "_"; [iNext;iExists w;iFrame|iModIntro].
-      iClear "HJmpRes".
       iApply wp_pure_step_later; auto.
       iNext; iIntros "_".
-
       iApply "Hexec" ; iFrame "∗ #".
       rewrite insert_commute //=.
       repeat (iSplit ; try done).
 
     - (* Success true *)
       rewrite insert_insert in HincrPC; subst regs'.
-      case_decide as HallowJmp.
+      match goal with
+      | H: _ |- context[(if (decide ?cond) then _ else _)]=>
+          destruct_decide (decide cond) as HallowJmp
+      end; auto.
       { (* contradiction *)
         rewrite /reg_allows_IE_jmp in HallowJmp.
-        destruct HallowJmp as ((Hregs0 & -> & Hwb & Hwb') & _ & _).
-        simplify_eq.
+        destruct HallowJmp as ((Hregs0 & -> & Hwb & Hwb') & _).
+        rewrite Hregs0 in Hdst.
+        simplify_map_eq.
       }
       iModIntro.
-      iDestruct "HJmpMem" as "(_&_&->)". rewrite -memMap_resource_1.
+      iDestruct "HJmpMem" as "->". rewrite -memMap_resource_1.
       iMod ("Hcls" with "[Hmem HP]") as "_";[iExists w;iFrame|iModIntro].
       iApply wp_pure_step_later; auto.
 
@@ -706,14 +354,18 @@ Section fundamental.
       rewrite insert_insert in Hregs'; subst regs'.
       simplify_map_eq.
 
-      case_decide as Heq; simplify_eq.
+      match goal with
+      | H: _ |- context [(if (decide ?cond) then _ else _)] =>
+          destruct_decide (decide cond) as Heq
+      end; simplify_eq.
       { (* contradiction *)
         exfalso.
-        destruct Heq as (_& H' & Hnz) ; simplify_eq.
-        congruence.
+        destruct Heq as (_ & Hnz) ; simplify_eq.
+        apply Hnz in HVsrc.
+        rewrite HVsrc in Hcond; congruence.
       }
       iModIntro.
-      iDestruct "HJmpMem" as "(_& %H' & ->)"; simplify_eq. rewrite -memMap_resource_1.
+      iDestruct "HJmpMem" as "->"; simplify_eq. rewrite -memMap_resource_1.
       iMod ("Hcls" with "[Hmem HP]") as "_";[iExists w;iFrame|iModIntro].
       iApply wp_pure_step_later; auto.
 
